

## Solo Project Derivations

### Solving the equation of radiative transfer

This solution follows that in Introduction to Stellar Astrophysics (E. Böhm-Vitense) pages 30-35 (Reference 7 in bibliography)

$$\frac{1}{\kappa_\lambda} \frac{dI_\lambda}{ds_\lambda} = -I_\lambda + S_\lambda$$

$$d\tau_\lambda = \kappa_\lambda ds$$

$$\Rightarrow \frac{dI_\lambda}{d\tau_\lambda} = -I_\lambda + S_\lambda$$

Multiplying by integrating factor  $e^{\tau_\lambda}$

$$\Rightarrow \frac{d(I_\lambda e^{\tau_\lambda})}{d\tau_\lambda} = S_\lambda e^{\tau_\lambda}$$

$$\Rightarrow \frac{d}{d\tau_\lambda} (I_\lambda e^{\tau_\lambda}) = S_\lambda e^{\tau_\lambda}$$

$$\Rightarrow \int_0^{\tau_\lambda} \frac{d}{d\tau_\lambda} (I_\lambda e^{\tau_\lambda}) d\tau_\lambda = \int_0^{\tau_\lambda} S_\lambda e^{\tau_\lambda} d\tau_\lambda$$

$$\Rightarrow [I_\lambda e^{\tau_\lambda}]_0^{\tau_\lambda} = [S_\lambda e^{\tau_\lambda}]_0^{\tau_\lambda}$$

$$I_\lambda e^{\tau_\lambda} - I_{\lambda 0} = S_\lambda e^{\tau_\lambda} - S_\lambda$$

assuming  $S_\lambda$  constant along  $\tau_\lambda$ .

$$\Rightarrow I_\lambda - I_{\lambda 0} e^{-\tau_\lambda} = S_\lambda (1 - e^{-\tau_\lambda})$$

$$\Rightarrow I_\lambda = I_{\lambda 0} e^{-\tau_\lambda} + S_\lambda (1 - e^{-\tau_\lambda})$$

If  $\tau_\lambda \ll 1$ ,  $e^{-\tau_\lambda} \approx 1 - \tau_\lambda$  (can expand the exponential in a Taylor series).

$$\begin{aligned}
 \Rightarrow I_{\lambda} &= I_{\lambda 0} (1 - \tau_{\lambda}) + S_{\lambda} (1 - (1 - \tau_{\lambda})) \\
 &= I_{\lambda 0} - I_{\lambda 0} \tau_{\lambda} + S_{\lambda} - S_{\lambda} + S_{\lambda} \tau_{\lambda} \\
 &= I_{\lambda 0} + \tau_{\lambda} (S_{\lambda} - I_{\lambda 0})
 \end{aligned}$$

If  $\tau_{\lambda} \gg 1$ ,  $e^{-\tau_{\lambda}} \rightarrow 0$

$$\Rightarrow I_{\lambda} = S_{\lambda}$$

Finding the wavelength of light emitted at the peak of the Sun's spectrum

By Wien's Law (Reference 12 in bibliography)

$$\lambda_{\text{peak}} = \frac{2.898 \times 10^{-3} \text{ mK}}{6000 \text{ K}}$$

$$\lambda_{\text{peak}} = 4.83 \times 10^{-7} \text{ m} \times \frac{1 \text{ cm}}{0.01 \text{ m}}$$

$$= 4.83 \times 10^{-5} \text{ cm}$$

$$= 483.3 \times 10^{-7} \text{ cm}$$

(as shown in the report).